Data for diploma thesis evaluation and fixed names for diploma thesis

Examples/diplomarbeit/evalLogs.py
@@ -1,0 +1,174 @@
+import pandas as pd
+import json
+
+def treeDepth(tree):
+    if tree["children"] is []:
+        return 1
+    else:
+        currdepth = 0
+        for child in tree["children"]:
+            depth = treeDepth(child)
+            if depth > currdepth:
+                currdepth = depth
+        return currdepth + 1
+    
+def treeNumNodes(tree):
+    numNodes = 1
+    for child in tree["node"]["children"]:
+        numNodes = numNodes + treeNumNodes(child)
+    return numNodes
+
+def graphNumNodes(graph):
+    vertices = set()
+
+    for e in graph["edges"]:
+        vertex = json.dumps(e["vertex"])
+        if  vertex in vertices:
+            pass
+        else:
+            vertices.add(vertex)
+        
+        for succ in e["successors"]:
+            succ = json.dumps(succ)
+            if succ in vertices:
+                pass
+            else:
+                vertices.add(succ)
+    return len(vertices)
+
+
+def evalExponentialExample():
+    columns = ["Type", "Size", "Number of nodes", "Nemo time", "Preparation time", "Validation time"]
+
+    df = pd.DataFrame(columns=columns)
+    outputs = set()
+    rows = []
+    with open("ExponentialTCLog.txt", "r") as log:
+        for line in log:
+            data = json.loads(line)
+            if data["type"] == "tree":
+                numberNodes = 0
+                for tree in data["problem"]:
+                    numberNodes = numberNodes + treeNumNodes(tree)
+            else:
+                numberNodes = graphNumNodes(data["problem"])
+            rows.append({"Type": data["type"], "Size": data["size"], "Number of nodes": int(numberNodes), "Nemo time": float(data["Nemo time"]), "Preparation time": float(data["Preparation time"]), "Validation time": float(data["Validation time"])})
+
+            if data["Result"] in outputs:
+                pass
+            else:
+                outputs.add(data["Result"])
+            df = pd.DataFrame(rows, index = list(range(0, len(rows))))
+
+            groupedDf = df.groupby(["Type", "Size"]).agg({"Number of nodes": ["mean"] , "Nemo time": ["mean", "std"], "Preparation time": ["mean", "std"], "Validation time": ["mean", "std"]})
+
+            groupedDf = groupedDf.style.format(precision=2)
+            print(outputs)
+            with open("Output.txt", "w") as output:
+                output.write(groupedDf.to_latex())
+
+def evalGraph():
+    columns = ["Type", "Density", "Completeness", "Number of nodes", "Preparation time", "Validation time"]
+
+    df = pd.DataFrame(columns=columns)
+    outputs = set()
+    rows = []
+    with open("log_graph.txt", "r") as log:
+        for line in log:
+            data = json.loads(line)
+            if data["Type"] == "tree":
+                numberNodes = 0
+                for tree in data["trees"]:
+                    numberNodes = numberNodes + treeNumNodes(tree)
+            else:
+                numberNodes = graphNumNodes(data["graph"])
+            rows.append({"Type": data["Type"], "Density": data["density"], "Completeness": data["completeness"], "Number of nodes": int(numberNodes), "Preparation time": float(data["Preparation time"]), "Validation time": float(data["Validation time"])})
+
+            if data["Result"] in outputs:
+                pass
+            else:
+                outputs.add(data["Result"])
+            df = pd.DataFrame(rows, index = list(range(0, len(rows))))
+            df.style.format(precision=2)
+
+            groupedDf = df.groupby(["Type", "Completeness", "Density"]).agg({"Number of nodes": ["mean", "std"], "Preparation time": ["mean", "std"], "Validation time": ["mean", "std"]})
+
+            groupedDf = groupedDf.style.format(precision=2)
+            print(outputs)
+            with open("Output.txt", "w") as output:
+                output.write(groupedDf.to_latex())
+
+def evalGalen():
+    columns = ["Type", "Number of nodes", "Nemo time", "Preparation time", "Validation time"]
+
+    df = pd.DataFrame(columns=columns)
+    outputs = set()
+    rows = []
+    with open("log_galen.txt", "r") as log:
+        for line in log:
+            data = json.loads(line)
+
+            if "trees" in data.keys():
+                numberNodes = 0
+                for tree in data["trees"]:
+                    numberNodes = numberNodes + treeNumNodes(tree)
+                    rowType = "tree"
+            else:
+                numberNodes = graphNumNodes(data["graph"])
+                rowType="graph"
+
+
+            rows.append({"Type": rowType, "Number of nodes": int(numberNodes), "Number of atoms": data["numberAtoms"], "Preparation time": float(data["Preparation time"]), "Validation time": float(data["Validation time"])})
+
+            if data["Result"] in outputs:
+                pass
+            else:
+                outputs.add(data["Result"])
+            df = pd.DataFrame(rows, index = list(range(0, len(rows))))
+
+            groupedDf = df.groupby(["Type", "Number of atoms"]).agg({"Number of nodes": ["mean", "std"], "Preparation time": ["mean", "std"], "Validation time": ["mean", "std"]})
+
+            groupedDf = groupedDf.style.format(precision=2)
+            print(outputs)
+            with open("Output.txt", "w") as output:
+                output.write(groupedDf.to_latex())
+
+
+def evalGraph2():
+    columns = ["Type", "Density", "Completeness", "Number of nodes", "Preparation time", "Validation time"]
+
+    df = pd.DataFrame(columns=columns)
+    outputs = set()
+    rows = []
+    with open("log_graph2.txt", "r") as log:
+        for line in log:
+            data = json.loads(line)
+            if data["Type"] == "tree":
+                numberNodes = 0
+                for tree in data["trees"]:
+                    numberNodes = numberNodes + treeNumNodes(tree)
+            else:
+                numberNodes = graphNumNodes(data["graph"])
+            if data["Rule file"] == "tc.rls":
+                programType = "A"
+            else:
+                programType = "B"
+                
+
+            rows.append({"Type": data["Type"], "Density": data["density"], "Program type": programType, "Number of nodes": int(numberNodes), "Preparation time": float(data["Preparation time"]), "Validation time": float(data["Validation time"])})
+
+            if data["Result"] in outputs:
+                pass
+            else:
+                outputs.add(data["Result"])
+            df = pd.DataFrame(rows, index = list(range(0, len(rows))))
+            df.style.format(precision=2)
+
+            groupedDf = df.groupby(["Type", "Program type", "Density"]).agg({"Number of nodes": ["mean", "std"], "Preparation time": ["mean", "std"], "Validation time": ["mean", "std"]})
+
+            groupedDf = groupedDf.style.format(precision=2)
+            print(outputs)
+            with open("Output.txt", "w") as output:
+                output.write(groupedDf.to_latex())
+
+evalGraph()
